src/Horizontal.ec
@@ -1,0 +1,1379 @@
+require import AllCore List SmtMap Distr IntExtra IntDiv DMap FSet.
+
+require import ALanguage ASecretSharingScheme AProtocolLibrary AAPI ASPSemantics AMPSemantics.
+require import MPCProtocolLibrary ProtocolAPI SPAPISemantics MPAPISemantics.
+require import MPProtocolAPISemantics.
+require import Utils.
+
+import SS.
+import MPCLib.
+import MPCAPI.
+
+theory Compilation.
+
+clone import Language as L.
+
+clone import MultiPartyProtocolAPISemantics as Source with
+ type L1.L = L,
+ type L2.L = L,
+ type L3.L = L.
+
+clone import Language as L1'.
+clone import Language as L2'.
+clone import Language as L3'.
+
+clone import MultiPartyProtocolAPISemantics as Target with
+  type L1.L = L1'.L,
+  type L2.L = L2'.L,
+  type L3.L = L3'.L.
+import MultiPartyAPISemantics.
+
+(* The REAL API *)
+module API_Real : API.API_t = {
+var senv: (svar_t, sharedValue_t) fmap
+proc init(): unit = {
+  senv <- empty;
+}
+proc nparties(): int = { return SecretSharingScheme.n; }
+proc declass(a: svar_t): (value_t * sideInfo_t) option = {
+  var vtr, r;
+   r <- None;
+   if (a \in senv) {
+    vtr <@ APIsec.prot_declass(oget senv.[a]);
+     r <- Some vtr;
+   }
+  return r;
+}
+proc input(a : svar_t, inp: sharedValue_t): sideInfo_t option = {
+  var tr;
+   tr <@ APIsec.prot_in(inp);
+  senv <- senv.[ a <- inp ];
+  return Some tr;
+}
+proc output(a: svar_t): (sharedValue_t * sideInfo_t) option = {
+  var o, tr, r;
+   r <- None;
+   if (a \in senv) {
+     (o, tr) <@ APIsec.prot_out(oget (senv.[a]));
+     r <- Some (o, tr);
+   }
+  return r;
+}
+proc sop(sop: MPCLib.sop_t, pargs: value_t list, sargs: svar_t list, a : svar_t) : sideInfo_t option = {
+  var r, tr, y;
+   r <- None;
+   if (forall x, x \in sargs /\ x \in senv) {
+     (y, tr) <@ APIsec.prot_sop(sop,pargs, map (fun x => oget senv.[x]) sargs);
+     senv <- senv.[ a <- y ];
+     r <- Some tr;
+   }
+  return r;
+}
+}.
+
+import MultiPartySemantics.
+
+lemma nosmt stepP_spec_h i st':
+   hoare [ ProgSem(API_Real).stepP :
+           id = i /\ ProgSem.st = st'
+          ==>
+           ProgSem.st = (if i = P1 then 
+                          {| st' with StP1 = oget (SemP1.stepPiter SemP1.stepL (b2i res) (st'.`StP1)) |}
+                        else if i = P2 then
+                          {| st' with StP2 = oget (SemP2.stepPiter SemP2.stepL (b2i res) (st'.`StP2)) |}
+                        else 
+                          {| st' with StP3 = oget (SemP3.stepPiter SemP3.stepL (b2i res) (st'.`StP3)) |}) /\
+           res = if i = P1 then (SemP1.stepPiter SemP1.stepL 1 (st'.`StP1) <> None)
+                 else if i = P2 then (SemP2.stepPiter SemP2.stepL 1 (st'.`StP2) <> None)
+                 else (SemP3.stepPiter SemP3.stepL 1 (st'.`StP3) <> None)
+         ].
+proof.
+proc. 
+case (i = P1).
+wp; skip; progress.
+rewrite /upd_Sigma1 => //=.
+congr.
+rewrite /b2i => /=.
+rewrite SemP1.stepPiter1.
+done.
+smt().
+rewrite SemP1.stepPiter1.
+done.
+smt().
+rewrite /b2i => /=. 
+rewrite SemP1.stepPiter0 => /=.
+done.
+smt().
+rewrite SemP1.stepPiter1.
+done.
+smt().
+rewrite /b2i => /=. 
+rewrite SemP1.stepPiter0 => /=.
+done.
+smt().
+smt(SemP1.callSt_stepPiter).
+case (i = P2).
+wp; skip; progress.
+rewrite /upd_Sigma2 => //=.
+congr.
+rewrite /b2i => /=.
+rewrite SemP2.stepPiter1.
+done.
+smt().
+rewrite SemP2.stepPiter1.
+done.
+smt().
+rewrite /b2i => /=. 
+rewrite SemP2.stepPiter0 => /=.
+done.
+smt().
+rewrite SemP2.stepPiter1.
+done.
+smt().
+rewrite /b2i => /=. 
+rewrite SemP2.stepPiter0 => /=.
+done.
+smt().
+smt(SemP2.callSt_stepPiter).
+case (i = P3).
+wp; skip; progress.
+rewrite /upd_Sigma3 => //=.
+congr.
+rewrite /b2i => /=.
+rewrite SemP3.stepPiter1.
+done.
+smt().
+rewrite SemP3.stepPiter1.
+done.
+smt().
+rewrite /b2i => /=. 
+rewrite SemP3.stepPiter0 => /=.
+done.
+smt().
+rewrite SemP3.stepPiter1.
+done.
+smt().
+rewrite /b2i => /=. 
+rewrite SemP3.stepPiter0 => /=.
+done.
+smt().
+smt(SemP3.callSt_stepPiter).
+exfalso => /#.
+qed.
+
+lemma nosmt stepP_ll: islossless ProgSem(API_Real).stepP.
+proof. by proc; wp; skip; progress => /#. qed.
+
+lemma nosmt stepP_spec i st': 
+  phoare [ ProgSem(API_Real).stepP :
+           id = i /\ ProgSem.st = st'
+          ==>
+           ProgSem.st = (if i = P1 then 
+                          {| st' with StP1 = oget (SemP1.stepPiter SemP1.stepL (b2i res) (st'.`StP1)) |}
+                        else if i = P2 then
+                          {| st' with StP2 = oget (SemP2.stepPiter SemP2.stepL (b2i res) (st'.`StP2)) |}
+                        else 
+                          {| st' with StP3 = oget (SemP3.stepPiter SemP3.stepL (b2i res) (st'.`StP3)) |}) /\
+           res = if i = P1 then (SemP1.stepPiter SemP1.stepL 1 (st'.`StP1) <> None)
+                 else if i = P2 then (SemP2.stepPiter SemP2.stepL 1 (st'.`StP2) <> None)
+                 else (SemP3.stepPiter SemP3.stepL 1 (st'.`StP3) <> None)
+         ] = 1%r.
+proof. by conseq stepP_ll (stepP_spec_h i st'). qed.
+
+(** COMPILERS **)
+
+(* Compiler Correctness *)
+
+(* equivalence relation on source/target local states *)
+op equivLSt ['ls, 'es, 'lt, 'et] : ('ls*'es) -> ('lt*'et) -> bool.
+
+print SemP1.API.apiCallRes.
+print API.apiCallRes.
+print ProtocolAPI.API.apiCallRes.
+print apiCallRes.
+
+op equivSt1 ['ls, 'es, 'lt, 'et] (s:('ls,'es) Source.MultiPartyAPISemantics.SemP1.APIst) (s':('lt,'et) Target.MultiPartyAPISemantics.SemP1.APIst) =
+ s.`1 = s'.`1 /\ equivLSt s.`2 s'.`2.
+op equivSt2 ['ls, 'es, 'lt, 'et] (s:('ls,'es) Source.MultiPartyAPISemantics.SemP2.APIst) (s':('lt,'et) Target.MultiPartyAPISemantics.SemP2.APIst) =
+ s.`1 = s'.`1 /\ equivLSt s.`2 s'.`2.
+op equivSt3 ['ls, 'es, 'lt, 'et] (s:('ls,'es) Source.MultiPartyAPISemantics.SemP3.APIst) (s':('lt,'et) Target.MultiPartyAPISemantics.SemP3.APIst) =
+ s.`1 = s'.`1 /\ equivLSt s.`2 s'.`2.
+
+lemma equivSt_callSt1 ['ls, 'es, 'lt, 'et]
+ (s1: ('ls, 'es) Source.MultiPartyAPISemantics.SemP1.APIst) (s2: ('lt, 'et) Target.MultiPartyAPISemantics.SemP1.APIst):
+ equivSt1 s1 s2 => SemP1.callSt s1 = SemP1.callSt s2.
+proof.
+by rewrite /equivSt /callSt; move => [-> _].
+qed.
+lemma equivSt_callSt2 ['ls, 'es, 'lt, 'et]
+ (s1: ('ls, 'es) Source.MultiPartyAPISemantics.SemP2.APIst) (s2: ('lt, 'et) Target.MultiPartyAPISemantics.SemP2.APIst):
+ equivSt2 s1 s2 => SemP2.callSt s1 = SemP2.callSt s2.
+proof.
+by rewrite /equivSt /callSt; move => [-> _].
+qed.
+lemma equivSt_callSt3 ['ls, 'es, 'lt, 'et]
+ (s1: ('ls, 'es) Source.MultiPartyAPISemantics.SemP3.APIst) (s2: ('lt, 'et) Target.MultiPartyAPISemantics.SemP3.APIst):
+ equivSt3 s1 s2 => SemP3.callSt s1 = SemP3.callSt s2.
+proof.
+by rewrite /equivSt /callSt; move => [-> _].
+qed.
+
+(* compilers *)
+op compiler1 : L.L -> L1.L.
+op compiler2 : L.L -> L2.L.
+op compiler3 : L.L -> L3.L.
+
+(* ASSUMPTION: equivalence of initial states *)
+axiom equivSt_init1 (P:L.L):
+  equivSt1 (Source.MultiPartyAPISemantics.SemP1.initSt (Source.MultiPartyAPISemantics.SemP1.initStateL P)) (Target.MultiPartyAPISemantics.SemP1.initSt (Target.MultiPartyAPISemantics.SemP1.initStateL (compiler1 P))).
+axiom equivSt_init2 (P:L.L):
+  equivSt2 (Source.MultiPartyAPISemantics.SemP2.initSt (Source.MultiPartyAPISemantics.SemP2.initStateL P)) (Target.MultiPartyAPISemantics.SemP2.initSt (Target.MultiPartyAPISemantics.SemP2.initStateL (compiler2 P))).
+axiom equivSt_init3 (P:L.L):
+  equivSt3 (Source.MultiPartyAPISemantics.SemP3.initSt (Source.MultiPartyAPISemantics.SemP3.initStateL P)) (Target.MultiPartyAPISemantics.SemP3.initSt (Target.MultiPartyAPISemantics.SemP3.initStateL (compiler3 P))).
+
+(* ASSUMPTION: backward simulation (trace preservation) *)
+axiom bisim_backward1 ss st kt st':
+ equivSt1 ss st =>
+ Target.MultiPartyAPISemantics.SemP1.stepPiter Target.MultiPartyAPISemantics.SemP1.stepL kt st = Some st' =>
+ Target.MultiPartyAPISemantics.SemP1.callSt st' <> None =>
+ (exists ks ss', Source.MultiPartyAPISemantics.SemP1.stepPiter Source.MultiPartyAPISemantics.SemP1.stepL ks ss = Some ss'
+                 /\ equivSt1 ss' st' /\ 0 <= ks).
+
+axiom bisim_backward2 ss st kt st':
+ equivSt2 ss st =>
+ Target.MultiPartyAPISemantics.SemP2.stepPiter Target.MultiPartyAPISemantics.SemP2.stepL kt st = Some st' =>
+ Target.MultiPartyAPISemantics.SemP2.callSt st' <> None =>
+ (exists ks ss', Source.MultiPartyAPISemantics.SemP2.stepPiter Source.MultiPartyAPISemantics.SemP2.stepL ks ss = Some ss'
+                 /\ equivSt2 ss' st' /\ 0 <= ks).
+
+axiom bisim_backward3 ss st kt st':
+ equivSt3 ss st =>
+ Target.MultiPartyAPISemantics.SemP3.stepPiter Target.MultiPartyAPISemantics.SemP3.stepL kt st = Some st' =>
+ Target.MultiPartyAPISemantics.SemP3.callSt st' <> None =>
+ (exists ks ss', Source.MultiPartyAPISemantics.SemP3.stepPiter Source.MultiPartyAPISemantics.SemP3.stepL ks ss = Some ss'
+                 /\ equivSt3 ss' st' /\ 0 <= ks).
+
+(* handling different paces among parties *)
+op advSt1 ['l,'e] step (ss: (L,Source.MultiPartyAPISemantics.SemP1.EnvL) Source.MultiPartyAPISemantics.SemP1.APIst) (st: ('l,'e) Target.MultiPartyAPISemantics.SemP1.APIst) : bool =
+ exists n st', 0 <= n /\ equivSt1 ss st' /\ Target.MultiPartyAPISemantics.SemP1.stepPiter step n st' = Some st.
+
+lemma advS01 ['l, 'e] step s1 (s2: ('l, 'e) Target.MultiPartyAPISemantics.SemP1.APIst):
+ equivSt1 s1 s2 => advSt1 step s1 s2.
+proof.
+move=> *; exists 0 s2; progress.
+by rewrite Target.MultiPartyAPISemantics.SemP1.stepPiter0.
+qed.
+
+lemma nosmt advSt_callSt1 ['l, 'e] step s1 (s2: ('l, 'e) Target.MultiPartyAPISemantics.SemP1.APIst):
+ advSt1 step s1 s2 =>
+ Target.MultiPartyAPISemantics.SemP1.callSt s1 <> None =>
+ equivSt1 s1 s2.
+proof.
+move=> [k st'] /> *.
+have ?: Target.MultiPartyAPISemantics.SemP1.callSt st' <> None by smt().
+move: (Target.MultiPartyAPISemantics.SemP1.callSt_stepPiter step k st' H4); move=> [?|?].
+ by move: H2; rewrite Target.MultiPartyAPISemantics.SemP1.stepPiter0 //.
+by move: H2; rewrite H5.
+qed.
+
+op advSt2 ['l,'e] step (ss: (L,Source.MultiPartyAPISemantics.SemP2.EnvL) Source.MultiPartyAPISemantics.SemP2.APIst) (st: ('l,'e) Target.MultiPartyAPISemantics.SemP2.APIst) : bool =
+ exists n st', 0 <= n /\ equivSt2 ss st' /\ Target.MultiPartyAPISemantics.SemP2.stepPiter step n st' = Some st.
+
+lemma advS02 ['l, 'e] step s1 (s2: ('l, 'e) Target.MultiPartyAPISemantics.SemP2.APIst):
+ equivSt1 s1 s2 => advSt1 step s1 s2.
+proof.
+move=> *; exists 0 s2; progress.
+by rewrite Target.MultiPartyAPISemantics.SemP2.stepPiter0.
+qed.
+
+lemma nosmt advSt_callSt2 ['l, 'e] step s1 (s2: ('l, 'e) Target.MultiPartyAPISemantics.SemP2.APIst):
+ advSt2 step s1 s2 =>
+ Target.MultiPartyAPISemantics.SemP2.callSt s1 <> None =>
+ equivSt2 s1 s2.
+proof.
+move=> [k st'] /> *.
+have ?: Target.MultiPartyAPISemantics.SemP2.callSt st' <> None by smt().
+move: (Target.MultiPartyAPISemantics.SemP2.callSt_stepPiter step k st' H4); move=> [?|?].
+ by move: H2; rewrite Target.MultiPartyAPISemantics.SemP2.stepPiter0 //.
+by move: H2; rewrite H5.
+qed.
+
+op advSt3 ['l,'e] step (ss: (L,Source.MultiPartyAPISemantics.SemP3.EnvL) Source.MultiPartyAPISemantics.SemP3.APIst) (st: ('l,'e) Target.MultiPartyAPISemantics.SemP3.APIst) : bool =
+ exists n st', 0 <= n /\ equivSt3 ss st' /\ Target.MultiPartyAPISemantics.SemP3.stepPiter step n st' = Some st.
+
+lemma advS03 ['l, 'e] step s1 (s2: ('l, 'e) Target.MultiPartyAPISemantics.SemP3.APIst):
+ equivSt3 s1 s2 => advSt3 step s1 s2.
+proof.
+move=> *; exists 0 s2; progress.
+by rewrite Target.MultiPartyAPISemantics.SemP3.stepPiter0.
+qed.
+
+lemma nosmt advSt_callSt3 ['l, 'e] step s1 (s2: ('l, 'e) Target.MultiPartyAPISemantics.SemP3.APIst):
+ advSt3 step s1 s2 =>
+ Target.MultiPartyAPISemantics.SemP3.callSt s1 <> None =>
+ equivSt3 s1 s2.
+proof.
+move=> [k st'] /> *.
+have ?: Target.MultiPartyAPISemantics.SemP3.callSt st' <> None by smt().
+move: (Target.MultiPartyAPISemantics.SemP3.callSt_stepPiter step k st' H4); move=> [?|?].
+ by move: H2; rewrite Target.MultiPartyAPISemantics.SemP3.stepPiter0 //.
+by move: H2; rewrite H5.
+qed.
+
+(*module RealSemMT: RealSemInterface = {
+  module PSem = ProgSemMT(API_Real)
+  include PSem
+}.*)
+
+module RealSemMT = Target.ProgSem(API_Real).
+
+module AdvOrclMT (Sem: AdvSemInterface) : AdvSemInterface = {
+  (* Simulator runs a local copy of all parties... *)
+  module SemEmu = RealSemMT
+  include SemEmu [- init, stepP, stepS]
+
+  proc init(P1:L1.L, P2:L2.L, P3:L3.L): unit = {
+    SemEmu.init(P1,P2,P3);
+  }
+  (* [stepP] relies on the local [RealSemMT] module in order to
+     control the execution of each party.
+     It leaves [Sem] untouched *)
+  proc stepP = SemEmu.stepP
+  (* Step Secret *)
+  proc stepS(): sideInfo_t option = {
+    var b, i, v;
+    var r <- None;
+    var ecall <- Target.syncPoint (Target.MultiPartyAPISemantics.SemP1.callSt (StP1 SemEmu.st),
+                            Target.MultiPartyAPISemantics.SemP2.callSt (StP2 SemEmu.st),
+                            Target.MultiPartyAPISemantics.SemP3.callSt (StP3 SemEmu.st));
+    if (ecall <> None) { (* call to the API *)
+      (* advance the source into a sync-point *)
+      i <- 0;
+      b <- true;
+      while (b) {
+        b <@  Sem.stepP(P1);
+        b <@  Sem.stepP(P2);
+        b <@  Sem.stepP(P3);
+        i <- i + 1;
+      }
+      (* do a [stepS] at the source *)
+      r <@ Sem.stepS();
+      if (r <> None) {
+          match (oget ecall) with
+          | Call_declass a => { v <- leakage_value (oget (oget r).`leakage);
+                                (* updates API result *)
+                                RealSemMT.st <- upd_SigmaAPI (Some (oget v)) RealSemMT.st;
+                              }
+          | Call_in a => { RealSemMT.st <- upd_SigmaAPI None RealSemMT.st; (* resets call *)
+                         }
+          | Call_out a => { RealSemMT.st <- upd_SigmaAPI None RealSemMT.st; (* resets call *)
+                          }
+      | Call_sop o a pargs sargs => { RealSemMT.st <- upd_SigmaAPI None RealSemMT.st; (* resets call *)
+                                    }
+      end;
+      }        
+    }
+    return r;
+  }
+}.
+
+section MTSecurityProof.
+
+declare module A: Adversary{ProgSem, ProgSem, AdvOrclMT}.
+declare module Z: Environment{A, API_Real, ProgSem, AdvOrclMT}.
+
+op inv (stMT1 stMT2: GlobalMTSt) (stST2: GlobalSt) =
+ stMT2.`P1 = stMT1.`P1 /\
+ stMT2.`P2 = stMT1.`P2 /\
+ stMT2.`P3 = stMT1.`P3 /\
+ stST2.`ib = stMT1.`ibmt /\
+ stST2.`ob = stMT1.`obmt /\
+ stST2.`Sigma.[1] <> None /\
+ stST2.`Sigma.[2] = stST2.`Sigma.[1] /\
+ stST2.`Sigma.[3] = stST2.`Sigma.[1] /\
+ advSt stepL1 (oget stST2.`Sigma.[1]) stMT1.`P1 /\
+ advSt stepL2 (oget stST2.`Sigma.[1]) stMT1.`P2 /\
+ advSt stepL3 (oget stST2.`Sigma.[1]) stMT1.`P3.
+
+local lemma nosmt stepP_prop:
+ equiv [ RealSemMT.stepP ~ AdvOrclMT(RealSem).stepP:
+         ={id} /\ ={API_Real.senv} /\
+         inv ProgSemMT.st{1} ProgSemMT.st{2} ProgSem.st{2}
+         ==>
+         ={res} /\ ={API_Real.senv} /\
+         inv ProgSemMT.st{1} ProgSemMT.st{2} ProgSem.st{2} ].
+proof.
+proc; wp; skip; rewrite /inv; progress.
+- smt(). smt(). smt(). smt(). smt(). smt(). smt(). smt().
+- move: H7 => [??[?[??]]].
+  exists (n+1) st'; progress; rewrite /upd_P1 /=; first smt().
+  apply: (stepPiterS_some _ _ _ _ _ _ H15) => //=.
+  by rewrite -some_oget //.
+- smt(). smt(). smt(). smt(). smt(). smt(). smt(). smt().
+  smt(). smt(). smt().
+- move: H8 => [??[?[??]]].
+  exists (n+1) st'; progress; rewrite /upd_P2 /=; first smt().
+  apply: (stepPiterS_some _ _ _ _ _ _ H16) => //=.
+  by rewrite -some_oget //.
+- smt(). smt(). smt(). smt(). smt(). smt(). smt(). smt().
+  smt(). smt(). smt().
+- move: H9 => [??[?[??]]].
+  exists (n+1) st'; progress; rewrite /upd_P3 /=; first smt().
+  apply: (stepPiterS_some _ _ _ _ _ _ H17) => //=.
+  by rewrite -some_oget //.
+- smt(). smt(). smt().
+qed.
+
+local lemma nosmt stepS_prop:
+ equiv [ RealSemMT.stepS ~ AdvOrclMT(RealSem).stepS:
+         true /\ ={API_Real.senv} /\
+         inv ProgSemMT.st{1} ProgSemMT.st{2} ProgSem.st{2}
+         ==>
+         ={res} /\ ={API_Real.senv} /\
+         inv ProgSemMT.st{1} ProgSemMT.st{2} ProgSem.st{2} ].
+proof.
+proc.
+sp 2 2; simplify.
+if; [smt() | | by skip; progress].
+seq 0 0: ((exists ks ss',
+            stepPiter stepL ks (oget ProgSem.st{2}.`Sigma.[1])
+            = Some ss' /\
+            equivSt ss' ProgSemMT.st{1}.`P1 /\ 0 <= ks)
+          /\ #[/:]pre).
+ skip; rewrite /inv => |> *.
+ move: H7 => [??[?[??]]].
+ apply (bisim_backward1 _ _ _ _ H11 H12 _); smt(). 
+elim* => ??.
+exists* (oget ProgSem.st{2}.`Sigma.[1]); elim* => ss.
+conseq (_: ss = oget ProgSem.st{2}.`Sigma.[1] /\
+           stepPiter stepL ks ss = Some ss' /\
+           equivSt ss' ProgSemMT.st{1}.`P1 /\
+           equivSt ss' ProgSemMT.st{1}.`P2 /\
+           equivSt ss' ProgSemMT.st{1}.`P3 /\
+           ={r,ecall,API_Real.senv} /\
+           0 <= ks /\ r{2}=None /\
+           ecall{2} = callSt ProgSemMT.st{2}.`P1 /\
+           ecall{2} = callSt ProgSemMT.st{2}.`P2 /\
+           ecall{2} = callSt ProgSemMT.st{2}.`P3 /\
+           ecall{2} <> None /\
+           ProgSemMT.st{2}.`P1 = ProgSemMT.st{1}.`P1 /\
+           ProgSemMT.st{2}.`P2 = ProgSemMT.st{1}.`P2 /\
+           ProgSemMT.st{2}.`P3 = ProgSemMT.st{1}.`P3 /\
+           ProgSem.st{2}.`ib = ProgSemMT.st{1}.`ibmt /\
+           ProgSem.st{2}.`ob = ProgSemMT.st{1}.`obmt /\
+           ProgSem.st{2}.`Sigma.[1] <> None /\
+           ProgSem.st{2}.`Sigma.[2] = ProgSem.st{2}.`Sigma.[1] /\
+           ProgSem.st{2}.`Sigma.[3] = ProgSem.st{2}.`Sigma.[1]
+           ==> _).
+ rewrite /inv => |> *; auto.
+ split; [|split; [|smt()]].
+  move: H11 => [??[?[??]]].
+  move: (bisim_backward2 _ _ _ _ H14 H15 _); first smt().
+  move=> [??] [?[??]].
+  have ?:= (stepPiter_det _ _ _ _ _ _ _ _ H _ H16 _); first 4 smt().
+  by move: H16; rewrite -H19 H; move => /#.
+ move: H12 => [??[?[??]]].
+ move: (bisim_backward3 _ _ _ _ H14 H15 _); first smt().
+ move=> [??] [?[??]].
+ have ?:= (stepPiter_det _ _ _ _ _ _ _ _ H _ H16 _); first 4 smt().
+ by move: H16; rewrite -H19 H; move => /#.
+seq 0 3: (ss' = (oget ProgSem.st{2}.`Sigma.[1]) /\
+          #[/3:]pre).          
+ sp 0 2.
+ while {2} ((b = (i <= ks)){2} /\
+             0 <= i{2} <= ks+1 /\ 
+             (stepPiter stepL ks ss = Some ss') /\
+             (stepPiter stepL (i+b2i b-1) ss = ProgSem.st{2}.`Sigma.[1]){2} /\
+             #[/5:]pre
+            ) (ks+1-i{2}).
+   move=> *; exlim ProgSem.st => sw.
+   case (i = ks).
+    wp; call (stepP_spec 3 sw).
+    call (stepP_spec 2 sw). 
+    call (stepP_spec 1 sw).
+    skip=> *.
+    have Hloop: stepPiter stepL 1 (oget ProgSem.st{hr}.`Sigma.[1])
+                = None.
+     move: H; progress.
+     move: H2; rewrite H18 b2i1 /= H1 => <- /=.
+     by move: (callSt_stepPiter stepL 1 ss' _); smt().
+    move: H; rewrite /inv;
+    progress; 1..6,8..: smt(stepPiter0 get_set_id).
+    - rewrite !H17 Hloop b2i0 /=; smt(get_setE).
+   wp; call (stepP_spec 3 
+    {| sw with Sigma = sw.`Sigma.[
+        1 <- oget (stepPiter stepL 1 (oget (sw.`Sigma.[1])))].[
+        2 <- oget (stepPiter stepL 1 (oget (sw.`Sigma.[1])))] |}).
+   call (stepP_spec 2 {| sw with Sigma = sw.`Sigma.[
+        1 <- oget (stepPiter stepL 1 (oget (sw.`Sigma.[1])))] |}). 
+   call (stepP_spec 1 sw).
+   skip => *.
+   have Hloop: stepPiter stepL 1 (oget ProgSem.st{hr}.`Sigma.[1])
+               <> None.
+    apply (stepPiter_lt _ ks i{hr} ss); first 2 smt().
+    rewrite -some_oget 1:/#.
+    move: H; progress; smt().
+   move: H; rewrite /inv; progress; 1..7,9..12: smt(get_setE).
+   - rewrite !get_setE /=.
+     rewrite H17 Hloop b2i1 /= -some_oget //.
+     rewrite stepPiterS; first smt().
+     move: H2; rewrite H18 b2i1 /= => ->.
+     by rewrite (some_oget ProgSem.st{hr}.`Sigma.[1]) /#.
+ skip; progress; 1..2,4..5: smt().
+ by rewrite b2i1 /= stepPiter0 // -some_oget /#.
+inline RealSem.stepS.
+seq 0 2: (#[/:]pre /\ r0{2} = None /\ ecall{1}=ecall0{2}).
+ wp; skip; rewrite /inv; progress.
+ rewrite /allECalls (_:3 = 1+1+1) 1:// !iotaS // iota1 /=.
+ by rewrite !H12 !H13 /= H3 (equivSt_callSt _ _ H) /#.
+rcondt {2} 1; first by move=>*; skip; progress.
+match; move=> *. 
+- (* call_declass *)
+  split; move => [a Ha]; exists a; smt().
+- (* call_in *)
+  split; move => [a Ha]; exists a; smt().
+- (* call_out *)
+  split; move => [a Ha]; exists a; smt().
+- (* call_sop *)
+  split; move => [o a pargs sargs Ho]; exists o a pargs sargs; smt().
+- (* call_declass *)
+  inline API_Real.api_declass.
+  rcondt {2} 7.
+   move=> *; inline*; wp; rnd; wp; skip; progress; smt().
+  inline*; sp.
+  seq 1 1: (#pre /\ ={t0}); first by rnd; skip; progress; smt().
+  sp; match {2}.
+  + move=> *; wp; skip; progress; first 5 smt().
+    - by rewrite /upd_SigmaAPI /= mapE /= /updRes /upd_ib /=
+                 (some_oget st_R.`Sigma.[1]) // /#.
+    - by rewrite /upd_SigmaAPI /upd_ib /= !mapE /= /#.
+    - by rewrite /upd_SigmaAPI /upd_ib /= !mapE /= /#.
+    - exists 0 (upd_P_API (Some (oget (leakage_value (oget t0{2}.`leakage)))) st_L).`P1.
+      split; first done.
+      split; last by apply stepPiter0.
+      by rewrite /equivSt /upd_P_API /upd_SigmaAPI
+                 /= mapE /= /updRes /= oget_omap_some /#.
+    - exists 0 (upd_P_API (Some (oget (leakage_value (oget t0{2}.`leakage)))) st_L).`P2.
+      split; first done.
+      split; last by apply stepPiter0.
+      by rewrite /equivSt /upd_P_API /upd_SigmaAPI
+                 /= mapE /= /updRes /= oget_omap_some /#.
+    - exists 0 (upd_P_API (Some (oget (leakage_value (oget t0{2}.`leakage)))) st_L).`P3.
+      split; first done.
+      split; last by apply stepPiter0.
+      by rewrite /equivSt /upd_P_API /upd_SigmaAPI
+                 /= mapE /= /updRes /= oget_omap_some /#.
+  + move=> *; wp; skip; progress; smt().
+  + move=> *; wp; skip; progress; smt().
+  + move=> *; wp; skip; progress; smt().
+- (* call_in *)
+  if => //=; [smt() | |]; last first.
+   rcondf {2} 2; first by move=>*; wp; skip; progress.
+   by wp; skip; progress; smt(advSt0).
+  seq 1 1: (#pre /\ ={t}).
+   call (_: ={API_Real.senv} /\ a{1}=a0{2}).
+    by inline*; wp; rnd; wp; skip; progress.
+   by skip; progress; smt().
+  rcondt {2} 5; first by move=>*; wp; skip; progress.
+  sp; match {2}; move=> *.
+  + wp; skip; progress; smt().
+  + wp; skip; rewrite /inv => |>*; progress; first 3 smt().
+    - by rewrite /upd_SigmaAPI /= mapE /= /updRes /upd_ib /=
+                 (some_oget st_R.`Sigma.[1]) // /#.
+    - by rewrite /upd_SigmaAPI /upd_ib /= !mapE /= /#.
+    - by rewrite /upd_SigmaAPI /upd_ib /= !mapE /= /#.
+    - exists 0 (upd_P_API None (upd_ibmt None st_L)).`P1.
+      split; first done.
+      split; last by rewrite stepPiter0.
+      by rewrite /equivSt /upd_P_API /upd_ibmt /upd_SigmaAPI
+                 /= mapE /= /upd_ib /= /updRes /= get_some /#.
+    - exists 0 (upd_P_API None (upd_ibmt None st_L)).`P2.
+      split; first done.
+      split; last by rewrite stepPiter0.
+      by rewrite /equivSt /upd_P_API /upd_ibmt /upd_SigmaAPI
+                 /= mapE /= /upd_ib /= /updRes /= get_some /#.
+    - exists 0 (upd_P_API None (upd_ibmt None st_L)).`P3.
+      split; first done.
+      split; last by rewrite stepPiter0.
+      by rewrite /equivSt /upd_P_API /upd_ibmt /upd_SigmaAPI
+                 /= mapE /= /upd_ib /= /updRes /= get_some /#.
+  + wp; skip; progress; smt().
+  + wp; skip; progress; smt().
+- (* call_out *)
+  if => //=; [smt() | |]; last first.
+   rcondf {2} 2; first by move=>*; wp; skip; progress.
+   by wp; skip; progress; smt(advSt0).
+  seq 1 1: (#pre /\ ={x, t}).
+   call (_: ={API_Real.senv} /\ a{1}=a0{2}).
+    by inline*; wp; rnd; wp; skip; progress.
+   by skip; progress; smt().
+  rcondt {2} 5; first by move=>*; wp; skip; progress.
+  sp; match {2}; move=> *.
+  + wp; skip; progress; smt().
+  + wp; skip; progress; smt().
+  + wp; skip; rewrite /inv => |>*; progress; first 3 smt().
+    - by rewrite /upd_SigmaAPI /upd_P_API /upd_obmt /= mapE /#.
+    - by rewrite /upd_SigmaAPI /upd_ob /= !mapE /= /#.
+    - by rewrite /upd_SigmaAPI /upd_ob /= !mapE /= /#.
+    - exists 0 (upd_P_API None (upd_ibmt None st_L)).`P1.
+      split; first done.
+      split; last by rewrite stepPiter0.
+      by rewrite /equivSt /upd_P_API /upd_ibmt /upd_SigmaAPI
+                 /= mapE /= /upd_ib /= /updRes /= get_some /#.
+    - exists 0 (upd_P_API None (upd_ibmt None st_L)).`P2.
+      split; first done.
+      split; last by rewrite stepPiter0.
+      by rewrite /equivSt /upd_P_API /upd_ibmt /upd_SigmaAPI
+                 /= mapE /= /upd_ib /= /updRes /= get_some /#.
+    - exists 0 (upd_P_API None (upd_ibmt None st_L)).`P3.
+      split; first done.
+      split; last by rewrite stepPiter0.
+      by rewrite /equivSt /upd_P_API /upd_ibmt /upd_SigmaAPI
+                 /= mapE /= /upd_ib /= /updRes /= get_some /#.
+  + wp; skip; progress; smt().
+- (* call_sop *)
+  seq 1 1: (#pre /\ ={t}).
+   call (_: ={API_Real.senv} /\
+            (o,pargs,sargs,a){1}=(o0,pargs0,sargs0,a0){2}).
+    by inline*; wp; rnd; wp; skip; progress.
+   by skip; progress; smt(advSt0).
+  rcondt {2} 4; first by move=>*; wp; skip; progress.
+  sp; match {2}; move=> *.
+  + wp; skip; progress; smt().
+  + wp; skip; progress; smt().
+  + wp; skip; progress; smt().
+  + wp; skip; rewrite /inv => |>*; progress; first 3 smt().
+    - rewrite /upd_SigmaAPI /= mapE /= /updRes /upd_ib /=
+              (some_oget st_R.`Sigma.[1]) // /#.
+    - by rewrite /upd_SigmaAPI /= !mapE /= /#.
+    - by rewrite /upd_SigmaAPI /= !mapE /= /#.
+    - exists 0 (upd_P_API None (upd_ibmt None st_L)).`P1.
+      split; first done.
+      split; last by rewrite stepPiter0.
+      by rewrite /equivSt /upd_P_API /upd_ibmt /upd_SigmaAPI
+                 /= mapE /= /upd_ib /= /updRes /= get_some /#.
+    - exists 0 (upd_P_API None (upd_ibmt None st_L)).`P2.
+      split; first done.
+      split; last by rewrite stepPiter0.
+      by rewrite /equivSt /upd_P_API /upd_ibmt /upd_SigmaAPI
+                 /= mapE /= /upd_ib /= /updRes /= get_some /#.
+    - exists 0 (upd_P_API None (upd_ibmt None st_L)).`P3.
+      split; first done.
+      split; last by rewrite stepPiter0.
+      by rewrite /equivSt /upd_P_API /upd_ibmt /upd_SigmaAPI
+                 /= mapE /= /upd_ib /= /updRes /= get_some /#.
+qed.
+
+
+equiv SecurityMT:
+ REAL_MT(Z, A).game ~ REAL(Z, AdvMT(A)).game
+ : ={P, glob A, glob Z} ==> ={res}.
+proof.
+proc.
+call (_: ={glob A, API_Real.senv} /\
+         inv ProgSemMT.st{1} ProgSemMT.st{2} ProgSem.st{2}
+     ). 
+- (* setInput *)
+  by proc; inline*; wp; skip; progress; smt().
+- (* getOutput *)
+  by proc; inline*; wp; skip; progress; smt().
+- (* activate *)
+  proc; call (_: ={API_Real.senv} /\
+                 inv ProgSemMT.st{1} ProgSemMT.st{2} ProgSem.st{2}
+             ).
+  + (* stepP *)
+    by apply stepP_prop.
+  + (* stepS *)
+    by apply stepS_prop.
+    by skip; progress. 
+- inline*; call (_: ={API_Real.senv} /\
+                    inv ProgSemMT.st{1} ProgSemMT.st{2} ProgSem.st{2}
+                ).
+  by apply stepP_prop.
+ by apply stepS_prop.
+wp; skip => /> *; progress.
+- rewrite /init_GlobalSt /= (_:3=1+1+1) 1:// !iotaS //= iota1 /=;
+  smt(get_setE).
+- rewrite /init_GlobalSt /= (_:3=1+1+1) 1:// !iotaS //= iota1 /=;
+  smt(get_setE).
+- rewrite /init_GlobalSt /= (_:3=1+1+1) 1:// !iotaS //= iota1 /=;
+  smt(get_setE).
+- rewrite /advStT; exists 0 (init_GlobalMTSt P{2}).`P1.
+  split; first done.
+  split; last by rewrite stepPiter0.
+  have ?:= (equivSt_init1 P{2}).
+  rewrite /init_GlobalSt /=  (_:3=1+1+1) 1:// !iotaS //= iota1 /=.
+  by rewrite !get_setE /#.
+- rewrite /advStT; exists 0 (init_GlobalMTSt P{2}).`P2.
+  split; first done.
+  split; last by rewrite stepPiter0.
+  have ?:= (equivSt_init2 P{2}).
+  rewrite /init_GlobalSt /=  (_:3=1+1+1) 1:// !iotaS //= iota1 /=.
+  by rewrite !get_setE /#.
+- rewrite /advStT; exists 0 (init_GlobalMTSt P{2}).`P3.
+  split; first done.
+  split; last by rewrite stepPiter0.
+  have ?:= (equivSt_init3 P{2}).
+  rewrite /init_GlobalSt /=  (_:3=1+1+1) 1:// !iotaS //= iota1 /=.
+  by rewrite !get_setE /#.
+qed.
+
+end section MTSecurityProof.
+
+
+
+
+
+
+
+
+
+
+
+
+
+
+
+
+
+
+
+
+
+
+
+end Compilation.
+
+
+
+theory MultiThreaded.
+
+clone import SingleThreaded as ST with op n_parties <- 3, op n_corrupted <- 3.
+
+(* Target Languages *)
+
+(* Programs *)
+type L1.
+type L2.
+type L3.
+
+(* Environment *)
+type EnvL1.
+type EnvL2.
+type EnvL3.
+
+(* initial state *)
+op initStateL1 (P:L1): L1*EnvL1.
+op initStateL2 (P:L2): L2*EnvL2.
+op initStateL3 (P:L3): L3*EnvL3.
+
+type StateL1 = (L1, EnvL1) APIst.
+type StateL2 = (L2, EnvL2) APIst.
+type StateL3 = (L3, EnvL3) APIst.
+
+(* (local) Step semantics *)
+op stepL1 : L1 -> EnvL1 -> apiRes_data option -> ((L1,EnvL1) ECall) option.
+op stepL2 : L2 -> EnvL2 -> apiRes_data option -> ((L2,EnvL2) ECall) option.
+op stepL3 : L3 -> EnvL3 -> apiRes_data option -> ((L3,EnvL3) ECall) option.
+
+
+(* ASSUMPTION: backward simulation (trace preservation) *)
+axiom bisim_backward1 ss st kt st':
+ equivSt ss st =>
+ stepPiter stepL1 kt st = Some st' =>
+ callSt st' <> None =>
+ (exists ks ss', stepPiter stepL ks ss = Some ss'
+                 /\ equivSt ss' st' /\ 0 <= ks).
+
+axiom bisim_backward2 ss st kt st':
+ equivSt ss st =>
+ stepPiter stepL2 kt st = Some st' =>
+ callSt st' <> None =>
+ (exists ks ss', stepPiter stepL ks ss = Some ss'
+                 /\ equivSt ss' st' /\ 0 <= ks).
+
+axiom bisim_backward3 ss st kt st':
+ equivSt ss st =>
+ stepPiter stepL3 kt st = Some st' =>
+ callSt st' <> None =>
+ (exists ks ss', stepPiter stepL ks ss = Some ss'
+                 /\ equivSt ss' st' /\ 0 <= ks).
+
+
+
+(* handling different paces among parties *)
+op advSt ['l,'e] step (ss: (L,EnvL) APIst) (st: ('l,'e) APIst) : bool =
+ exists n st', 0 <= n /\ equivSt ss st' /\ stepPiter step n st' = Some st.
+
+lemma advSt0 ['l, 'e] step s1 (s2: ('l, 'e) APIst):
+ equivSt s1 s2 => advSt step s1 s2.
+proof.
+move=> *; exists 0 s2; progress.
+by rewrite stepPiter0.
+qed.
+
+lemma nosmt advSt_callSt ['l, 'e] step s1 (s2: ('l, 'e) APIst):
+ advSt step s1 s2 =>
+ callSt s1 <> None =>
+ equivSt s1 s2.
+proof.
+move=> [k st'] /> *.
+have ?: callSt st' <> None by smt().
+move: (callSt_stepPiter step k st' H4); move=> [?|?].
+ by move: H2; rewrite stepPiter0 //.
+by move: H2; rewrite H5.
+qed.
+
+
+
+(* END languages *)
+
+
+
+
+(* Global state for the multi-target setting (every party uses the same language) *)
+type GlobalMTSt = { P1: StateL1
+                  ; P2: StateL2
+                  ; P3: StateL3
+                  ; ibmt: sharedValue_t option
+                  ; obmt: sharedValue_t option
+                  }.
+
+
+
+
+(* updates a local state after a [stepP] *)
+op upd_P1 (newst: (L1,EnvL1) ECall) (st: GlobalMTSt): GlobalMTSt=
+ {| st with P1 = st_from_step newst |}.
+op upd_P2 (newst: (L2,EnvL2) ECall) (st: GlobalMTSt): GlobalMTSt=
+ {| st with P2 = st_from_step newst |}.
+op upd_P3 (newst: (L3,EnvL3) ECall) (st: GlobalMTSt): GlobalMTSt=
+ {| st with P3 = st_from_step newst |}.
+(* updates all local states after a [stepS] *)
+op upd_P_API (r: apiRes_data option) (st: GlobalMTSt): GlobalMTSt =
+ {| st with P1 = updRes r (P1 st); P2 = updRes r (P2 st); P3 = updRes r (P3 st) |}.
+(* updates the input buffer *)
+op upd_ibmt (newib: sharedValue_t option) (st: GlobalMTSt): GlobalMTSt =
+ {| st with ibmt = newib |}.
+(* updates the output buffer *)
+op upd_obmt (newob: sharedValue_t option) (st: GlobalMTSt): GlobalMTSt =
+ {| st with obmt = newob |}.
+
+
+(* initial [GlobalMTSt] *)
+op init_GlobalMTSt (P: L) : GlobalMTSt =
+ {| P1 = iniSt (initStateL1 (compiler1 P))
+  ; P2 = iniSt (initStateL2 (compiler2 P))
+  ; P3 = iniSt (initStateL3 (compiler3 P))
+  ; ibmt = None
+  ; obmt = None
+ |}.
+
+module ProgSemMT (API: API_t) = {
+  var st: GlobalMTSt
+  proc init(P: L): unit = {
+    API.api_init();
+    st <- init_GlobalMTSt P;
+  }
+  (* Step Public *)
+  proc stepP(id: partyId_t): bool = {
+    var r <- false;
+    var newst1 <- stepL1 (progSt (P1 st)) (envSt (P1 st)) (resSt (P1 st));
+    var newst2 <- stepL2 (progSt (P2 st)) (envSt (P2 st)) (resSt (P2 st));
+    var newst3 <- stepL3 (progSt (P3 st)) (envSt (P3 st)) (resSt (P3 st));
+    if (id = 1 && callSt (P1 st) = None && newst1 <> None) {
+      r <- true;
+      st <- upd_P1 (oget newst1) st;
+    }
+    if (id = 2 && callSt (P2 st) = None && newst2 <> None) {
+      r <- true;
+      st <- upd_P2 (oget newst2) st;
+    }
+    if (id = 3 && callSt (P3 st) = None && newst3 <> None) {
+      r <- true;
+      st <- upd_P3 (oget newst3) st;
+    }
+    return r;
+  }
+  (* Step Secret *)
+  proc stepS(): sideInfo_t option = {
+    var x, v, t;
+    var r <- None;
+    var ecall <- syncPoint [callSt (P1 st); callSt (P2 st); callSt (P3 st)];
+    if (ecall <> None) { (* call to the API *)
+      match (oget ecall) with
+      | Call_declass a => { (v, t) <@ API.api_declass(a);
+                            r <- Some t;
+                            (* updates API result *)
+                            st <- upd_P_API (Some v) st;
+                          }
+      | Call_in a => { if (ibmt st <> None) {
+                         t <@ API.api_in(a, oget (ibmt st));
+                         r <- Some t;
+                         st <- upd_ibmt None st; (* clears buffer *)
+                         st <- upd_P_API None st; (* resets call *)
+                       }
+                     }
+      | Call_out a => { if (obmt st = None) {
+                          (x, t) <@ API.api_out(a);
+                          r <- Some t;
+                          st <- upd_obmt (Some x) st; (* fills buffer *)
+                          st <- upd_P_API None st; (* resets call *)
+                          }
+                      }
+      | Call_sop o a pargs sargs => { t <@ API.api_sop(o, pargs, sargs, a);
+                                      r <- Some t;
+                                      st <- upd_P_API None st; (* resets call *)
+                                    }
+      end;
+    }
+    return r;
+  }
+  proc setInput(x: sharedValue_t): bool = {
+    var r <- false;
+    if (ibmt st = None) {
+      r <- true;
+      st <- upd_ibmt (Some x) st;
+    }
+    return r;
+  }
+  proc getOutput(): sharedValue_t option = {
+    var r: sharedValue_t option;
+    r <- obmt st;
+    if (r <> None) {
+      st <- upd_obmt None st;
+    }
+    return r;
+  }
+}.
+
+
+
+module RealSemMT: RealSemInterface = {
+  module PSem = ProgSemMT(API_Real)
+  include PSem
+}.
+
+module AdvOrclMT (Sem: AdvSemInterface) : AdvSemInterface = {
+  (* Simulator runs a local copy of all parties... *)
+  module SemEmu = RealSemMT
+  include SemEmu [- init, stepP, stepS]
+
+  proc init(P:L): unit = {
+    SemEmu.init(P);
+  }
+  (* [stepP] relies on the local [RealSemMT] module in order to
+     control the execution of each party.
+     It leaves [Sem] untouched *)
+  proc stepP = SemEmu.stepP
+  (* Step Secret *)
+  proc stepS(): sideInfo_t option = {
+    var b, i, v;
+    var r <- None;
+    var ecall <- syncPoint [callSt (P1 SemEmu.PSem.st);
+                            callSt (P2 SemEmu.PSem.st);
+                            callSt (P3 SemEmu.PSem.st)];
+    if (ecall <> None) { (* call to the API *)
+      (* advance the source into a sync-point *)
+      i <- 0;
+      b <- true;
+      while (b) {
+        b <@  Sem.stepP(1);
+        b <@  Sem.stepP(2);
+        b <@  Sem.stepP(3);
+        i <- i + 1;
+      }
+      (* do a [stepS] at the source *)
+      r <@ Sem.stepS();
+      if (r <> None) {
+          match (oget ecall) with
+          | Call_declass a => { v <- leakage_value (oget (oget r).`leakage);
+                                (* updates API result *)
+                                RealSemMT.PSem.st <- upd_P_API (Some (oget v)) RealSemMT.PSem.st;
+                              }
+          | Call_in a => { RealSemMT.PSem.st <- upd_P_API None RealSemMT.PSem.st; (* resets call *)
+                         }
+          | Call_out a => { RealSemMT.PSem.st <- upd_P_API None RealSemMT.PSem.st; (* resets call *)
+                          }
+      | Call_sop o a pargs sargs => { RealSemMT.PSem.st <- upd_P_API None RealSemMT.PSem.st; (* resets call *)
+                                    }
+      end;
+      }        
+    }
+    return r;
+  }
+}.
+
+module AdvMT (A: AdvInterface) (S:AdvSemInterface) : AdvEnvInterface = {
+  module AdvO = AdvOrclMT(S)
+  module Adv = A(AdvO)
+  proc init(P: L): unit = {
+    AdvO.init(P);
+    Adv.init(P);
+  }
+  proc activate = Adv.activate
+}.
+
+module REAL_MT (E: Env) (A: AdvInterface) = {
+  module Sem = RealSemMT
+  module Adv = A(Sem)
+  module Z = E(EnvO(Sem, Adv))
+  proc game(P: L): bool = {
+    var b;
+    Sem.init(P);
+    Adv.init(P);
+    b <@ Z.animate();
+    return b;
+  }
+}.
+
+
+section MTSecurityProof.
+
+declare module A: AdvInterface{ProgSem, ProgSemMT, AdvOrclMT}.
+declare module Z: Env{A, API_Real, ProgSem, ProgSemMT, AdvOrclMT}.
+
+op inv (stMT1 stMT2: GlobalMTSt) (stST2: GlobalSt) =
+ stMT2.`P1 = stMT1.`P1 /\
+ stMT2.`P2 = stMT1.`P2 /\
+ stMT2.`P3 = stMT1.`P3 /\
+ stST2.`ib = stMT1.`ibmt /\
+ stST2.`ob = stMT1.`obmt /\
+ stST2.`Sigma.[1] <> None /\
+ stST2.`Sigma.[2] = stST2.`Sigma.[1] /\
+ stST2.`Sigma.[3] = stST2.`Sigma.[1] /\
+ advSt stepL1 (oget stST2.`Sigma.[1]) stMT1.`P1 /\
+ advSt stepL2 (oget stST2.`Sigma.[1]) stMT1.`P2 /\
+ advSt stepL3 (oget stST2.`Sigma.[1]) stMT1.`P3.
+
+local lemma nosmt stepP_prop:
+ equiv [ RealSemMT.stepP ~ AdvOrclMT(RealSem).stepP:
+         ={id} /\ ={API_Real.senv} /\
+         inv ProgSemMT.st{1} ProgSemMT.st{2} ProgSem.st{2}
+         ==>
+         ={res} /\ ={API_Real.senv} /\
+         inv ProgSemMT.st{1} ProgSemMT.st{2} ProgSem.st{2} ].
+proof.
+proc; wp; skip; rewrite /inv; progress.
+- smt(). smt(). smt(). smt(). smt(). smt(). smt(). smt().
+- move: H7 => [??[?[??]]].
+  exists (n+1) st'; progress; rewrite /upd_P1 /=; first smt().
+  apply: (stepPiterS_some _ _ _ _ _ _ H15) => //=.
+  by rewrite -some_oget //.
+- smt(). smt(). smt(). smt(). smt(). smt(). smt(). smt().
+  smt(). smt(). smt().
+- move: H8 => [??[?[??]]].
+  exists (n+1) st'; progress; rewrite /upd_P2 /=; first smt().
+  apply: (stepPiterS_some _ _ _ _ _ _ H16) => //=.
+  by rewrite -some_oget //.
+- smt(). smt(). smt(). smt(). smt(). smt(). smt(). smt().
+  smt(). smt(). smt().
+- move: H9 => [??[?[??]]].
+  exists (n+1) st'; progress; rewrite /upd_P3 /=; first smt().
+  apply: (stepPiterS_some _ _ _ _ _ _ H17) => //=.
+  by rewrite -some_oget //.
+- smt(). smt(). smt().
+qed.
+
+local lemma nosmt stepS_prop:
+ equiv [ RealSemMT.stepS ~ AdvOrclMT(RealSem).stepS:
+         true /\ ={API_Real.senv} /\
+         inv ProgSemMT.st{1} ProgSemMT.st{2} ProgSem.st{2}
+         ==>
+         ={res} /\ ={API_Real.senv} /\
+         inv ProgSemMT.st{1} ProgSemMT.st{2} ProgSem.st{2} ].
+proof.
+proc.
+sp 2 2; simplify.
+if; [smt() | | by skip; progress].
+seq 0 0: ((exists ks ss',
+            stepPiter stepL ks (oget ProgSem.st{2}.`Sigma.[1])
+            = Some ss' /\
+            equivSt ss' ProgSemMT.st{1}.`P1 /\ 0 <= ks)
+          /\ #[/:]pre).
+ skip; rewrite /inv => |> *.
+ move: H7 => [??[?[??]]].
+ apply (bisim_backward1 _ _ _ _ H11 H12 _); smt(). 
+elim* => ??.
+exists* (oget ProgSem.st{2}.`Sigma.[1]); elim* => ss.
+conseq (_: ss = oget ProgSem.st{2}.`Sigma.[1] /\
+           stepPiter stepL ks ss = Some ss' /\
+           equivSt ss' ProgSemMT.st{1}.`P1 /\
+           equivSt ss' ProgSemMT.st{1}.`P2 /\
+           equivSt ss' ProgSemMT.st{1}.`P3 /\
+           ={r,ecall,API_Real.senv} /\
+           0 <= ks /\ r{2}=None /\
+           ecall{2} = callSt ProgSemMT.st{2}.`P1 /\
+           ecall{2} = callSt ProgSemMT.st{2}.`P2 /\
+           ecall{2} = callSt ProgSemMT.st{2}.`P3 /\
+           ecall{2} <> None /\
+           ProgSemMT.st{2}.`P1 = ProgSemMT.st{1}.`P1 /\
+           ProgSemMT.st{2}.`P2 = ProgSemMT.st{1}.`P2 /\
+           ProgSemMT.st{2}.`P3 = ProgSemMT.st{1}.`P3 /\
+           ProgSem.st{2}.`ib = ProgSemMT.st{1}.`ibmt /\
+           ProgSem.st{2}.`ob = ProgSemMT.st{1}.`obmt /\
+           ProgSem.st{2}.`Sigma.[1] <> None /\
+           ProgSem.st{2}.`Sigma.[2] = ProgSem.st{2}.`Sigma.[1] /\
+           ProgSem.st{2}.`Sigma.[3] = ProgSem.st{2}.`Sigma.[1]
+           ==> _).
+ rewrite /inv => |> *; auto.
+ split; [|split; [|smt()]].
+  move: H11 => [??[?[??]]].
+  move: (bisim_backward2 _ _ _ _ H14 H15 _); first smt().
+  move=> [??] [?[??]].
+  have ?:= (stepPiter_det _ _ _ _ _ _ _ _ H _ H16 _); first 4 smt().
+  by move: H16; rewrite -H19 H; move => /#.
+ move: H12 => [??[?[??]]].
+ move: (bisim_backward3 _ _ _ _ H14 H15 _); first smt().
+ move=> [??] [?[??]].
+ have ?:= (stepPiter_det _ _ _ _ _ _ _ _ H _ H16 _); first 4 smt().
+ by move: H16; rewrite -H19 H; move => /#.
+seq 0 3: (ss' = (oget ProgSem.st{2}.`Sigma.[1]) /\
+          #[/3:]pre).          
+ sp 0 2.
+ while {2} ((b = (i <= ks)){2} /\
+             0 <= i{2} <= ks+1 /\ 
+             (stepPiter stepL ks ss = Some ss') /\
+             (stepPiter stepL (i+b2i b-1) ss = ProgSem.st{2}.`Sigma.[1]){2} /\
+             #[/5:]pre
+            ) (ks+1-i{2}).
+   move=> *; exlim ProgSem.st => sw.
+   case (i = ks).
+    wp; call (stepP_spec 3 sw).
+    call (stepP_spec 2 sw). 
+    call (stepP_spec 1 sw).
+    skip=> *.
+    have Hloop: stepPiter stepL 1 (oget ProgSem.st{hr}.`Sigma.[1])
+                = None.
+     move: H; progress.
+     move: H2; rewrite H18 b2i1 /= H1 => <- /=.
+     by move: (callSt_stepPiter stepL 1 ss' _); smt().
+    move: H; rewrite /inv;
+    progress; 1..6,8..: smt(stepPiter0 get_set_id).
+    - rewrite !H17 Hloop b2i0 /=; smt(get_setE).
+   wp; call (stepP_spec 3 
+    {| sw with Sigma = sw.`Sigma.[
+        1 <- oget (stepPiter stepL 1 (oget (sw.`Sigma.[1])))].[
+        2 <- oget (stepPiter stepL 1 (oget (sw.`Sigma.[1])))] |}).
+   call (stepP_spec 2 {| sw with Sigma = sw.`Sigma.[
+        1 <- oget (stepPiter stepL 1 (oget (sw.`Sigma.[1])))] |}). 
+   call (stepP_spec 1 sw).
+   skip => *.
+   have Hloop: stepPiter stepL 1 (oget ProgSem.st{hr}.`Sigma.[1])
+               <> None.
+    apply (stepPiter_lt _ ks i{hr} ss); first 2 smt().
+    rewrite -some_oget 1:/#.
+    move: H; progress; smt().
+   move: H; rewrite /inv; progress; 1..7,9..12: smt(get_setE).
+   - rewrite !get_setE /=.
+     rewrite H17 Hloop b2i1 /= -some_oget //.
+     rewrite stepPiterS; first smt().
+     move: H2; rewrite H18 b2i1 /= => ->.
+     by rewrite (some_oget ProgSem.st{hr}.`Sigma.[1]) /#.
+ skip; progress; 1..2,4..5: smt().
+ by rewrite b2i1 /= stepPiter0 // -some_oget /#.
+inline RealSem.stepS.
+seq 0 2: (#[/:]pre /\ r0{2} = None /\ ecall{1}=ecall0{2}).
+ wp; skip; rewrite /inv; progress.
+ rewrite /allECalls (_:3 = 1+1+1) 1:// !iotaS // iota1 /=.
+ by rewrite !H12 !H13 /= H3 (equivSt_callSt _ _ H) /#.
+rcondt {2} 1; first by move=>*; skip; progress.
+match; move=> *. 
+- (* call_declass *)
+  split; move => [a Ha]; exists a; smt().
+- (* call_in *)
+  split; move => [a Ha]; exists a; smt().
+- (* call_out *)
+  split; move => [a Ha]; exists a; smt().
+- (* call_sop *)
+  split; move => [o a pargs sargs Ho]; exists o a pargs sargs; smt().
+- (* call_declass *)
+  inline API_Real.api_declass.
+  rcondt {2} 7.
+   move=> *; inline*; wp; rnd; wp; skip; progress; smt().
+  inline*; sp.
+  seq 1 1: (#pre /\ ={t0}); first by rnd; skip; progress; smt().
+  sp; match {2}.
+  + move=> *; wp; skip; progress; first 5 smt().
+    - by rewrite /upd_SigmaAPI /= mapE /= /updRes /upd_ib /=
+                 (some_oget st_R.`Sigma.[1]) // /#.
+    - by rewrite /upd_SigmaAPI /upd_ib /= !mapE /= /#.
+    - by rewrite /upd_SigmaAPI /upd_ib /= !mapE /= /#.
+    - exists 0 (upd_P_API (Some (oget (leakage_value (oget t0{2}.`leakage)))) st_L).`P1.
+      split; first done.
+      split; last by apply stepPiter0.
+      by rewrite /equivSt /upd_P_API /upd_SigmaAPI
+                 /= mapE /= /updRes /= oget_omap_some /#.
+    - exists 0 (upd_P_API (Some (oget (leakage_value (oget t0{2}.`leakage)))) st_L).`P2.
+      split; first done.
+      split; last by apply stepPiter0.
+      by rewrite /equivSt /upd_P_API /upd_SigmaAPI
+                 /= mapE /= /updRes /= oget_omap_some /#.
+    - exists 0 (upd_P_API (Some (oget (leakage_value (oget t0{2}.`leakage)))) st_L).`P3.
+      split; first done.
+      split; last by apply stepPiter0.
+      by rewrite /equivSt /upd_P_API /upd_SigmaAPI
+                 /= mapE /= /updRes /= oget_omap_some /#.
+  + move=> *; wp; skip; progress; smt().
+  + move=> *; wp; skip; progress; smt().
+  + move=> *; wp; skip; progress; smt().
+- (* call_in *)
+  if => //=; [smt() | |]; last first.
+   rcondf {2} 2; first by move=>*; wp; skip; progress.
+   by wp; skip; progress; smt(advSt0).
+  seq 1 1: (#pre /\ ={t}).
+   call (_: ={API_Real.senv} /\ a{1}=a0{2}).
+    by inline*; wp; rnd; wp; skip; progress.
+   by skip; progress; smt().
+  rcondt {2} 5; first by move=>*; wp; skip; progress.
+  sp; match {2}; move=> *.
+  + wp; skip; progress; smt().
+  + wp; skip; rewrite /inv => |>*; progress; first 3 smt().
+    - by rewrite /upd_SigmaAPI /= mapE /= /updRes /upd_ib /=
+                 (some_oget st_R.`Sigma.[1]) // /#.
+    - by rewrite /upd_SigmaAPI /upd_ib /= !mapE /= /#.
+    - by rewrite /upd_SigmaAPI /upd_ib /= !mapE /= /#.
+    - exists 0 (upd_P_API None (upd_ibmt None st_L)).`P1.
+      split; first done.
+      split; last by rewrite stepPiter0.
+      by rewrite /equivSt /upd_P_API /upd_ibmt /upd_SigmaAPI
+                 /= mapE /= /upd_ib /= /updRes /= get_some /#.
+    - exists 0 (upd_P_API None (upd_ibmt None st_L)).`P2.
+      split; first done.
+      split; last by rewrite stepPiter0.
+      by rewrite /equivSt /upd_P_API /upd_ibmt /upd_SigmaAPI
+                 /= mapE /= /upd_ib /= /updRes /= get_some /#.
+    - exists 0 (upd_P_API None (upd_ibmt None st_L)).`P3.
+      split; first done.
+      split; last by rewrite stepPiter0.
+      by rewrite /equivSt /upd_P_API /upd_ibmt /upd_SigmaAPI
+                 /= mapE /= /upd_ib /= /updRes /= get_some /#.
+  + wp; skip; progress; smt().
+  + wp; skip; progress; smt().
+- (* call_out *)
+  if => //=; [smt() | |]; last first.
+   rcondf {2} 2; first by move=>*; wp; skip; progress.
+   by wp; skip; progress; smt(advSt0).
+  seq 1 1: (#pre /\ ={x, t}).
+   call (_: ={API_Real.senv} /\ a{1}=a0{2}).
+    by inline*; wp; rnd; wp; skip; progress.
+   by skip; progress; smt().
+  rcondt {2} 5; first by move=>*; wp; skip; progress.
+  sp; match {2}; move=> *.
+  + wp; skip; progress; smt().
+  + wp; skip; progress; smt().
+  + wp; skip; rewrite /inv => |>*; progress; first 3 smt().
+    - by rewrite /upd_SigmaAPI /upd_P_API /upd_obmt /= mapE /#.
+    - by rewrite /upd_SigmaAPI /upd_ob /= !mapE /= /#.
+    - by rewrite /upd_SigmaAPI /upd_ob /= !mapE /= /#.
+    - exists 0 (upd_P_API None (upd_ibmt None st_L)).`P1.
+      split; first done.
+      split; last by rewrite stepPiter0.
+      by rewrite /equivSt /upd_P_API /upd_ibmt /upd_SigmaAPI
+                 /= mapE /= /upd_ib /= /updRes /= get_some /#.
+    - exists 0 (upd_P_API None (upd_ibmt None st_L)).`P2.
+      split; first done.
+      split; last by rewrite stepPiter0.
+      by rewrite /equivSt /upd_P_API /upd_ibmt /upd_SigmaAPI
+                 /= mapE /= /upd_ib /= /updRes /= get_some /#.
+    - exists 0 (upd_P_API None (upd_ibmt None st_L)).`P3.
+      split; first done.
+      split; last by rewrite stepPiter0.
+      by rewrite /equivSt /upd_P_API /upd_ibmt /upd_SigmaAPI
+                 /= mapE /= /upd_ib /= /updRes /= get_some /#.
+  + wp; skip; progress; smt().
+- (* call_sop *)
+  seq 1 1: (#pre /\ ={t}).
+   call (_: ={API_Real.senv} /\
+            (o,pargs,sargs,a){1}=(o0,pargs0,sargs0,a0){2}).
+    by inline*; wp; rnd; wp; skip; progress.
+   by skip; progress; smt(advSt0).
+  rcondt {2} 4; first by move=>*; wp; skip; progress.
+  sp; match {2}; move=> *.
+  + wp; skip; progress; smt().
+  + wp; skip; progress; smt().
+  + wp; skip; progress; smt().
+  + wp; skip; rewrite /inv => |>*; progress; first 3 smt().
+    - rewrite /upd_SigmaAPI /= mapE /= /updRes /upd_ib /=
+              (some_oget st_R.`Sigma.[1]) // /#.
+    - by rewrite /upd_SigmaAPI /= !mapE /= /#.
+    - by rewrite /upd_SigmaAPI /= !mapE /= /#.
+    - exists 0 (upd_P_API None (upd_ibmt None st_L)).`P1.
+      split; first done.
+      split; last by rewrite stepPiter0.
+      by rewrite /equivSt /upd_P_API /upd_ibmt /upd_SigmaAPI
+                 /= mapE /= /upd_ib /= /updRes /= get_some /#.
+    - exists 0 (upd_P_API None (upd_ibmt None st_L)).`P2.
+      split; first done.
+      split; last by rewrite stepPiter0.
+      by rewrite /equivSt /upd_P_API /upd_ibmt /upd_SigmaAPI
+                 /= mapE /= /upd_ib /= /updRes /= get_some /#.
+    - exists 0 (upd_P_API None (upd_ibmt None st_L)).`P3.
+      split; first done.
+      split; last by rewrite stepPiter0.
+      by rewrite /equivSt /upd_P_API /upd_ibmt /upd_SigmaAPI
+                 /= mapE /= /upd_ib /= /updRes /= get_some /#.
+qed.
+
+
+equiv SecurityMT:
+ REAL_MT(Z, A).game ~ REAL(Z, AdvMT(A)).game
+ : ={P, glob A, glob Z} ==> ={res}.
+proof.
+proc.
+call (_: ={glob A, API_Real.senv} /\
+         inv ProgSemMT.st{1} ProgSemMT.st{2} ProgSem.st{2}
+     ). 
+- (* setInput *)
+  by proc; inline*; wp; skip; progress; smt().
+- (* getOutput *)
+  by proc; inline*; wp; skip; progress; smt().
+- (* activate *)
+  proc; call (_: ={API_Real.senv} /\
+                 inv ProgSemMT.st{1} ProgSemMT.st{2} ProgSem.st{2}
+             ).
+  + (* stepP *)
+    by apply stepP_prop.
+  + (* stepS *)
+    by apply stepS_prop.
+    by skip; progress. 
+- inline*; call (_: ={API_Real.senv} /\
+                    inv ProgSemMT.st{1} ProgSemMT.st{2} ProgSem.st{2}
+                ).
+  by apply stepP_prop.
+ by apply stepS_prop.
+wp; skip => /> *; progress.
+- rewrite /init_GlobalSt /= (_:3=1+1+1) 1:// !iotaS //= iota1 /=;
+  smt(get_setE).
+- rewrite /init_GlobalSt /= (_:3=1+1+1) 1:// !iotaS //= iota1 /=;
+  smt(get_setE).
+- rewrite /init_GlobalSt /= (_:3=1+1+1) 1:// !iotaS //= iota1 /=;
+  smt(get_setE).
+- rewrite /advStT; exists 0 (init_GlobalMTSt P{2}).`P1.
+  split; first done.
+  split; last by rewrite stepPiter0.
+  have ?:= (equivSt_init1 P{2}).
+  rewrite /init_GlobalSt /=  (_:3=1+1+1) 1:// !iotaS //= iota1 /=.
+  by rewrite !get_setE /#.
+- rewrite /advStT; exists 0 (init_GlobalMTSt P{2}).`P2.
+  split; first done.
+  split; last by rewrite stepPiter0.
+  have ?:= (equivSt_init2 P{2}).
+  rewrite /init_GlobalSt /=  (_:3=1+1+1) 1:// !iotaS //= iota1 /=.
+  by rewrite !get_setE /#.
+- rewrite /advStT; exists 0 (init_GlobalMTSt P{2}).`P3.
+  split; first done.
+  split; last by rewrite stepPiter0.
+  have ?:= (equivSt_init3 P{2}).
+  rewrite /init_GlobalSt /=  (_:3=1+1+1) 1:// !iotaS //= iota1 /=.
+  by rewrite !get_setE /#.
+qed.
+
+end section MTSecurityProof.
+
+
+end MultiThreaded.
+
+(*
+print MultiThreaded.SecurityMT.
+*)
